AwsCryptographicMaterialProviders/dafny/AwsCryptographicMaterialProviders/src/CMCs/StormTracker.dfy
@@ -25,25 +25,26 @@ module {:options "/functionSyntax:4" }  StormTracker {
   import Time
 
   datatype CacheState =
-    | RealEmpty // No data, client should wait
-    | FakeEmpty // No data, client should fetch
+    | EmptyWait // No data, client should wait
+    | EmptyFetch // No data, client should fetch
     | Full(data : Types.GetCacheEntryOutput)
 
   class StormTracker {
 
     ghost predicate ValidState()
-      reads this, Modifies
+      reads this, wrapped, wrapped.Modifies
     {
-      && this in Modifies
-      && wrapped in Modifies
-      && inFlight in Modifies
-      && wrapped.Modifies <= Modifies
+      // && this in Modifies
+      // && wrapped in Modifies
+      // && inFlight in Modifies
+      // && wrapped.Modifies <= Modifies
       && this !in wrapped.Modifies
+      && inFlight !in wrapped.Modifies
       && wrapped.ValidState()
     }
     var wrapped : LocalCMC.LocalCMC;
     var inFlight: MutableMap<seq<uint8>, Types.PositiveLong>
-    ghost var Modifies : set<object>
+    // ghost var Modifies : set<object>
 
     constructor(
       entryCapacity: nat,
@@ -51,16 +52,24 @@ module {:options "/functionSyntax:4" }  StormTracker {
     )
       requires entryPruningTailSize >= 1
       ensures
-        && this.wrapped.ValidState()
-        && fresh(this.Modifies)
+        && this.ValidState()
+        && fresh(this.wrapped)
+        && fresh(this.wrapped.Modifies)
+        && fresh(this.inFlight)
     {
       this.wrapped := new LocalCMC.LocalCMC(entryCapacity, entryPruningTailSize);
       this.inFlight := new MutableMap();
-      new;
-      Modifies := { wrapped, inFlight, this } + wrapped.Modifies;
+      // new;
+      // Modifies := { wrapped, inFlight, this } + wrapped.Modifies;
     }
 
-    // If entry is within 10 seconds of expiration, then return FakeEmpty once per second, 
+    ghost function Modifies() : set<object>
+      reads this, wrapped, wrapped.Modifies
+    {
+      {inFlight} + wrapped.Modifies
+    }
+
+    // If entry is within 10 seconds of expiration, then return EmptyFetch once per second, 
     // and return cached value otherwise
     method CheckInFlight(identifier: seq<uint8>, result: Types.GetCacheEntryOutput, now : Types.PositiveLong)
       returns (output: CacheState)
@@ -75,39 +84,41 @@ module {:options "/functionSyntax:4" }  StormTracker {
         assert 0 < timeLeft <= 10;
         if inFlight.HasKey(identifier) {
           var entry := inFlight.Select(identifier);
-          if entry <= timeLeft {  // already returned a FakeEmpty for this second
+          if entry <= timeLeft {  // already returned a EmptyFetch for this second
             return Full(result);
           }
         }
         inFlight.Put(identifier, timeLeft);
-        return FakeEmpty;
+        return EmptyFetch;
       }
     }
 
-    // If entry is not in cache, then return FakeEmpty once per second, and RealEmpty otherwise
+    // If entry is not in cache, then return EmptyFetch once per second, and EmptyWait otherwise
     method CheckNewEntry(identifier: seq<uint8>, now : Types.PositiveLong)
       returns (output: CacheState)
       modifies inFlight
     {
       if inFlight.HasKey(identifier) {
         var entry := inFlight.Select(identifier);
-        if entry == now {  // already returned a FakeEmpty for this second
-          return RealEmpty;
+        if entry == now {  // already returned a EmptyFetch for this second
+          return EmptyWait;
         }
       }
       inFlight.Put(identifier, now);
-      return FakeEmpty;
+      return EmptyFetch;
     }
 
     // Pass in timestamp for easier testing
     method GetFromCacheWithTime(input: Types.GetCacheEntryInput, now : Types.PositiveLong)
       returns (output: Result<CacheState, Types.Error>)
       requires ValidState()
-      modifies Modifies
-      decreases Modifies
+      modifies inFlight, wrapped.Modifies
       ensures ValidState()
+      ensures inFlight == old(inFlight)
+      ensures wrapped == old(wrapped)
+      ensures wrapped.Modifies <= old(wrapped.Modifies)
     {
-      var result := wrapped.GetCacheEntry'(input);
+      var result := wrapped.GetCacheEntryWithTime(input, now);
       if result.Success? {
         var newResult := CheckInFlight(input.identifier, result.value, now);
         return Success(newResult);
@@ -122,9 +133,11 @@ module {:options "/functionSyntax:4" }  StormTracker {
     method GetFromCache(input: Types.GetCacheEntryInput)
       returns (output: Result<CacheState, Types.Error>)
       requires ValidState()
-      modifies Modifies
-      decreases Modifies
+      modifies inFlight, wrapped.Modifies
       ensures ValidState()
+      ensures inFlight == old(inFlight)
+      ensures wrapped == old(wrapped)
+      ensures wrapped.Modifies <= old(wrapped.Modifies)
     {
       var now := Time.GetCurrent();
       output := GetFromCacheWithTime(input, now);
@@ -135,8 +148,7 @@ module {:options "/functionSyntax:4" }  StormTracker {
     method GetCacheEntry(input: Types.GetCacheEntryInput)
       returns (output: Result<Types.GetCacheEntryOutput, Types.Error>)
       requires ValidState()
-      modifies Modifies
-      decreases Modifies
+      modifies inFlight, wrapped.Modifies
       ensures ValidState()
     {
       var result := GetFromCache(input);
@@ -153,20 +165,20 @@ module {:options "/functionSyntax:4" }  StormTracker {
     method PutCacheEntry(input: Types.PutCacheEntryInput)
       returns (output: Result<(), Types.Error>)
       requires ValidState()
-      modifies Modifies
-      decreases Modifies
+      modifies inFlight, wrapped.Modifies
       ensures ValidState()
+      ensures inFlight == old(inFlight)
+      ensures wrapped == old(wrapped)
+      ensures fresh(wrapped.Modifies - old(wrapped.Modifies))
     {
       inFlight.Remove(input.identifier);
       output := wrapped.PutCacheEntry'(input);
-      Modifies := { wrapped, inFlight, this } + wrapped.Modifies;
     }
 
     method DeleteCacheEntry(input: Types.DeleteCacheEntryInput)
       returns (output: Result<(), Types.Error>)
       requires ValidState()
-      modifies Modifies
-      decreases Modifies
+      modifies inFlight, wrapped.Modifies
       ensures ValidState()
     {
       inFlight.Remove(input.identifier);
@@ -176,8 +188,7 @@ module {:options "/functionSyntax:4" }  StormTracker {
     method UpdaterUsageMetadata(input: Types.UpdaterUsageMetadataInput)
       returns (output: Result<(), Types.Error>)
       requires ValidState()
-      modifies Modifies
-      decreases Modifies
+      modifies inFlight, wrapped.Modifies
       ensures ValidState()
     {
       output := wrapped.UpdaterUsageMetadata'(input);
