AwsCryptographicMaterialProviders/dafny/AwsCryptographicMaterialProviders/src/CMCs/LocalCMC.dfy
@@ -362,13 +362,25 @@ module {:options "/functionSyntax:4" } LocalCMC {
       modifies Modifies - {History}
       decreases Modifies - {History}
       ensures ValidState()
-      // ensures output.Failure? ==> input.identifier !in cache
+      ensures GetCacheEntryEnsuresPublicly(input, output)
+      ensures unchanged(History)
+      ensures Modifies <= old(Modifies)
+    {
+      var now := Time.GetCurrent();
+      output := GetCacheEntryWithTime(input, now);
+    }
+
+    method GetCacheEntryWithTime(input: Types.GetCacheEntryInput, now : Types.PositiveLong)
+      returns (output: Result<Types.GetCacheEntryOutput, Types.Error>)
+      requires ValidState()
+      modifies Modifies - {History}
+      decreases Modifies - {History}
+      ensures ValidState()
       ensures GetCacheEntryEnsuresPublicly(input, output)
       ensures unchanged(History)
       ensures Modifies <= old(Modifies)
     {
       if input.identifier in cache.Keys() {
-        var now := Time.GetCurrent();
         var entry := cache.Select(input.identifier);
         //= aws-encryption-sdk-specification/framework/cryptographic-materials-cache.md#time-to-live-ttl
         //# After a cache entry's TTL has elapsed,
@@ -395,7 +407,7 @@ module {:options "/functionSyntax:4" } LocalCMC {
           //= aws-encryption-sdk-specification/framework/local-cryptographic-materials-cache.md#get-cache-entry
           //# When performing a Get Cache Entry operation,
           //# the local CMC MUST [prune TTL-expired cache entries](#pruning).
-          var _ :- pruning();
+          var _ :- pruning(now);
         } else {
           // We removed this key,
           // no need to garbage collect
@@ -580,7 +592,7 @@ module {:options "/functionSyntax:4" } LocalCMC {
     //# The local CMC SHOULD also periodically evict all TTL-expired entries
     //# among the `N` least recently used entries.
 
-    method pruning()
+    method pruning(now : Types.PositiveLong)
       returns (output: Result<(), Types.Error>)
       requires ValidState()
       modifies Modifies - {History}
@@ -589,8 +601,6 @@ module {:options "/functionSyntax:4" } LocalCMC {
       ensures unchanged(History)
       ensures Modifies <= old(Modifies)
     {
-
-      var now := Time.GetCurrent();
       //= aws-encryption-sdk-specification/framework/local-cryptographic-materials-cache.md#pruning
       //# To prune TTL-expired cache entries,
       //# the local CMC MUST evict all TTL-expired entries
