AwsCryptographicMaterialProviders/dafny/AwsCryptographicMaterialProviders/test/CMCs/StormTracker.dfy
@@ -1,0 +1,57 @@
+// Copyright Amazon.com Inc. or its affiliates. All Rights Reserved.
+// SPDX-License-Identifier: Apache-2.0
+
+include "../../src/Index.dfy"
+include "../TestUtils.dfy"
+
+module  {:options "/functionSyntax:4"} TestStormTracker {
+  import opened AwsCryptographyMaterialProvidersTypes
+  import opened UInt = StandardLibrary.UInt
+  import opened Wrappers
+  import opened StormTracker
+  import UTF8
+
+  function MakeMat(data : Utf8Bytes) : Materials
+  {
+    BranchKey(BranchKey := BranchKeyMaterials (
+                branchKeyVersion := data,
+                branchKey := data
+              ))
+  }
+
+  function MakeGet(data : Utf8Bytes) : GetCacheEntryInput
+  {
+    GetCacheEntryInput (
+      identifier := data,
+      bytesUsed := Option.None
+    )
+  }
+  function MakePut(data : Utf8Bytes, expiryTime : PositiveLong) : PutCacheEntryInput
+  {
+    PutCacheEntryInput (
+      identifier := data,
+      materials := MakeMat(data),
+      creationTime := 123456789,
+      expiryTime := expiryTime,
+      messagesUsed := Option.None,
+      bytesUsed := Option.None
+    )
+  }
+
+  method {:test} StormTrackerBasics() {
+    var st := new StormTracker(100);
+
+    var abc := UTF8.EncodeAscii("abc");
+    var cde := UTF8.EncodeAscii("cde");
+    var res :- expect st.GetFromCacheWithTime(MakeGet(abc), 10000);
+    expect res.EmptyFetch?;
+    res :- expect st.GetFromCacheWithTime(MakeGet(abc), 10000);
+    expect res.EmptyWait?;
+    var res2 :- expect st.PutCacheEntry(MakePut(abc, 10000));
+    res2 :- expect st.PutCacheEntry(MakePut(cde, 10000));
+    res :- expect st.GetFromCacheWithTime(MakeGet(abc), 10001);
+    expect res.EmptyFetch?;
+    res :- expect st.GetFromCacheWithTime(MakeGet(abc), 10001);
+    expect res.EmptyWait?;
+  }
+}
